Finish formula and predicate semantics
Use custom dependently typed list-like datatype
for arguments (which have different types)

proofs/core/Semantics.v
@@ -3,19 +3,51 @@ Require Import Syntax.
 
 (** Semantics **)
 
-Fixpoint curry (l: list Type) (ret: Type) : Type :=
-  match l with
-  | nil => ret
-  | x :: t => x -> (curry t ret)
+(*A custom list-like data type which holds values of types [[s_i]], where
+    s is a list of sorts*)
+Inductive arg_list (domain: sort -> Type) : list sort -> Type :=
+  | AL_nil: arg_list domain nil
+  | AL_cons: forall s tl,
+      domain s ->
+      arg_list domain tl ->
+      arg_list domain (s :: tl).
+
+(*Some definitions on [arg_list]*)
+Fixpoint arg_length {domain: sort -> Type} {l: list sort} (a: arg_list domain l) : nat :=
+  match a with
+  | AL_nil _ => 0
+  | AL_cons _ _ _ d tl => 1 + arg_length tl
   end.
+
+Lemma arg_length_sorts: forall (domain: sort -> Type) (l: list sort) (a: arg_list domain l),
+  arg_length a = length l.
+Proof.
+  intros d l a. induction a; simpl; auto.
+Qed.
+
+Definition arg_nth {domain: sort -> Type} {l: list sort} (a: arg_list domain l) (i: nat)
+  (Hi: i < length l) (d: sort) : domain (nth i l d).
+Proof.
+  rewrite <- (arg_length_sorts domain l a) in Hi.
+  generalize dependent i. induction a; simpl; intros.
+  - exfalso. apply (Nat.nlt_0_r i). apply Hi.
+    (*not using lia because it might be hard to compute*) 
+  - destruct i.
+    + simpl. apply d0.
+    + apply IHa. apply lt_S_n, Hi.
+Defined.
 
 (*Here, we prove that a type substitution that replaces all of the type
   parameters for a function/pred symbol with sorts results in a sort *)
-Definition subst_funsym_params (f: funsym) (s: list sort) 
+Definition funsym_sigma_args (f: funsym) (s: list sort) 
   (Hlen: length (s_params f) = length s): list sort :=
   ty_subst_list_s (s_params f) s Hlen (s_args f) (s_args_wf f).
 
-Definition subst_predsym_params (p: predsym) (s: list sort)
+Definition funsym_sigma_ret (f: funsym) (s: list sort)
+(Hlen: length (s_params f) = length s) : sort :=
+  ty_subst_s (s_params f) s Hlen (s_ret f) (s_ret_wf f).
+
+Definition predsym_sigma_args (p: predsym) (s: list sort)
   (Hlen: length (p_params p) = length s) : list sort :=
   ty_subst_list_s (p_params p) s Hlen (p_args p) (p_args_wf p).
 
@@ -27,11 +59,11 @@ Record pre_interp := {
   (*This is quite unwieldy (and could be wrong) - need to see if works/can do better*)
 
   funs: forall (f:funsym) (s: list sort) (Hlen: length (s_params f) = length s),
-    curry (map domain (subst_funsym_params f s Hlen))
-      (domain (ty_subst_s (s_params f) s Hlen (s_ret f) (s_ret_wf f)));
+    arg_list domain (funsym_sigma_args f s Hlen) ->
+    (domain (funsym_sigma_ret f s Hlen));
+
   preds: forall (p:predsym) (s: list sort) (Hlen: length (p_params p) = length s),
-    curry (map domain (subst_predsym_params p s Hlen))
-      Prop
+    arg_list domain (predsym_sigma_args p s Hlen) -> bool
 }.
 
 (*Substitute according to function*)
@@ -105,17 +137,41 @@ destruct (vty_eq_dec ty ty').
 - apply (v_vars i v (m - 1) ty').
 Defined.
 
-Definition bool_of_binop (b: binop) : bool -> bool -> bool :=
-  match b with
-  | Tand => andb
-  | Tor => orb
-  | Timplies => implb
-  | Tiff => eqb
-  end.
+(* Some additional lemmas for casting/dependent type obligations *)
+
+Lemma map_length_eq: forall {A B C: Type} (f: B -> C) (l1 : list A) (l2 : list B),
+  length l1 = length l2 ->
+  length l1 = length (map f l2).
+Proof.
+  intros. rewrite H, map_length. reflexivity.
+Qed.
+
+(* If we have a sort, then substituting a valuation does nothing *)
+Lemma subst_sort_eq: forall (s: sort) (v: typevar -> sort),
+  s = v_subst v (sort_to_ty s).
+Proof.
+  intros. unfold v_subst. destruct s.
+  induction x; simpl; auto; try solve[apply sort_inj; reflexivity].
+  - apply sort_inj; simpl. unfold is_sort in i0. simpl in i0. inversion i0.
+  - rewrite Forall_forall in H. apply sort_inj; simpl.
+    f_equal. apply list_eq_ext'; try rewrite !map_length; auto.
+    intros n d Hn. rewrite map_nth_inbound with(d2:=d); auto.
+    assert (Hin: In (nth n vs d) vs) by (apply nth_In; auto).
+    assert (Hsort: is_sort (nth n vs d)). {
+      unfold is_sort. unfold is_sort in i0.
+      rewrite (type_vars_cons tsym vs); auto. 
+      destruct (type_vars (vty_cons tsym vs)) eqn : Ht; auto. inversion i0.
+    }
+    specialize (H _ Hin Hsort). inversion H. reflexivity.
+Qed. 
+
+(*Cast 1 domain into another*)
+Definition dom_cast (v1 v2: sort) (Hv: v1 = v2) (x: domain i v1) : domain i v2.
+subst. apply x.
+Defined.
+
 
 (* Semantics/Interpretation *)
-(*Difficulty - should only be defined for well-typed terms - will we need
-  dependent types?*)
 
 (*TODO: is the underlying logic supposed to be classical or constructive?
   Seemingly classical in paper because formula interpretations are equal to bool.
@@ -124,6 +180,14 @@ Definition bool_of_binop (b: binop) : bool -> bool -> bool :=
 
 (* We use bools rather than Props to better match the intended semantics in
    in the paper. As a bonus, we get proof irrelevance for free. *)
+
+Definition bool_of_binop (b: binop) : bool -> bool -> bool :=
+  match b with
+  | Tand => andb
+  | Tor => orb
+  | Timplies => implb
+  | Tiff => eqb
+  end.
 
 Inductive term_interp: 
   forall (v: valuation i) (tm: term) (ty: vty) (x: domain i (v_subst (v_typevar i v) ty)), Prop :=
@@ -146,11 +210,45 @@ Inductive term_interp:
     term_interp v t1 ty1 x1 ->
     term_interp (substi v ty1 x1) t2 ty2 x2 ->
     term_interp v (Tlet t1 ty1 t2) ty2 x2
-  (*| TI_func: forall v (f: funsym) (params: list vty) (ts: list term) ty xs x,
-    let tys := ty_subst_list (s_params f) params  
-    Forall (fun x => term_interp v (fst x) (snd x)) (combine (combine (s_args ) ts xs) ->
-    term_interp v *)
-  (*Only 1 left: function TODO: I think we need sorts for this*)
+  | TI_func: forall (v: valuation i) (f: funsym) (params: list vty) (ts: list term) 
+    (Hlen: length (s_params f) = length params) xs,
+
+    let v_map := v_subst (v_typevar i v) in
+    (* First, we get the interpretation of f *)
+    let f_interp := (funs i) f (map v_map params) 
+      (map_length_eq v_map _ _ Hlen) in
+    (* Return type of f (sigma(s_ret f))*)
+    let f_ret := (funsym_sigma_ret f (map v_map params) 
+      (map_length_eq v_map _ _ Hlen)) in
+    (*Now we need to apply it to the arguments*)
+    (*argument ts_i has type sigma((s_args f)_i), where sigma is
+      the map that sends the function params alpha_i -> v(params_i).
+      This means that all of these types are sorts, so v(sigma(s_args f)_i) =
+      sigma((s_args f)_i). Therefore, if [[t_i]]_v = x_i, x_i has the correct
+      type to pass into f_interp. However, we need manual casting in Coq
+      and this gets quite ugly. *)
+
+    (*The list of sigma(s_args)_i*)
+    let f_arg_typs : list sort :=
+      funsym_sigma_args f (map v_map params) (map_length_eq v_map _ _ Hlen) in
+
+    (*ith elt of xs is [[t_i]]_v. We need to cast the types to get the type as
+      [[v(sigma(s_args f)_i)]]*)
+    (* We give 0 and s_int as the default term and sort, respectively. This is
+       arbitrary and doesn't matter, our length assumptions ensures everything is
+       within bounds.*)
+    (forall n (Hn: n < length f_arg_typs),
+      (*Ignoring dependent type obligations/casting, this says that:
+        For all n in bounds, [nth n ts] (of type [nth n f_args_typs]) 
+        evaluates to [nth xs n] under v *)
+      term_interp v (nth n ts (Tconst (ConstInt 0)))
+        (nth n f_arg_typs s_int) 
+        (dom_cast _ _ (subst_sort_eq (nth n f_arg_typs s_int) (v_typevar i v)) 
+          (@arg_nth _ f_arg_typs xs n Hn s_int))) ->
+    
+    (*Again, we must cast the return type of f, for the same reason*)
+    term_interp v (Tfun f params ts) f_ret 
+      (dom_cast _ _ (subst_sort_eq f_ret (v_typevar i v)) (f_interp xs))
 
 with formula_interp: (valuation i) -> formula -> bool -> Prop :=
   | FI_true: forall v, formula_interp v Ftrue true
@@ -196,8 +294,36 @@ with formula_interp: (valuation i) -> formula -> bool -> Prop :=
     term_interp v t2 ty x2 ->
     x1 <> x2 ->
     formula_interp v (Feq ty t1 t2) false
+  | FI_prop: forall (v: valuation i) (p: predsym) (params: list vty) (ts: list term) 
+    (Hlen: length (p_params p) = length params) xs,
+
+    (*Very similar to function*)
+
+    let v_map := v_subst (v_typevar i v) in
+    (* First, we get the interpretation of p *)
+    let p_interp := (preds i) p (map v_map params) 
+      (map_length_eq v_map _ _ Hlen) in
+    (*let f_ret := (funsym_sigma_ret f (map v_map params) 
+      (map_length_eq v_map _ _ Hlen)) in*)
+
+    (*The list of sigma(s_args)_i*)
+    let p_arg_typs : list sort :=
+      predsym_sigma_args p (map v_map params) (map_length_eq v_map _ _ Hlen) in
+    (*ith elt of xs is [[t_i]]_v. We need to cast the types to get the type as
+      [[v(sigma(s_args f)_i)]]*)
+
+    (forall n (Hn: n < length p_arg_typs),
+      term_interp v (nth n ts (Tconst (ConstInt 0)))
+        (nth n p_arg_typs s_int) 
+        (dom_cast _ _ (subst_sort_eq (nth n p_arg_typs s_int) (v_typevar i v)) 
+          (@arg_nth _ p_arg_typs xs n Hn s_int))) ->
+
+    formula_interp v (Fpred p params ts) (p_interp xs)
     .
-(*TODO: functions and predicates*)
+
+(* Tests/Examples *)
+
+(*Our rules for quantifiers are OK constructively*)
 
 Lemma test1: forall {A: Type} (P: A -> Prop),
   (forall x, ~(P x)) ->
