proofs/core/Common.v
@@ -2,6 +2,7 @@ Require Export Coq.Lists.List.
 Require Export Coq.Bool.Bool.
 Export ListNotations.
 Require Import Coq.Logic.Eqdep_dec.
+Require Import Lia.
 (** Generally useful definitions, lemmas, and tactics *)
 
 (** Working with bool/props **)
@@ -83,6 +84,16 @@ Proof.
       exfalso. apply n0. rewrite IHl1 in i. apply in_remove in i. destruct i; auto.
 Qed.
 
+Lemma union_nil: forall (l1 l2: list A),
+  union l1 l2 = nil ->
+  l1 = nil /\ l2 = nil.
+Proof.
+  intros. induction l1; simpl; auto.
+  simpl in H. destruct (in_dec eq_dec a (union l1 l2)).
+  - rewrite H in i. inversion i.
+  - inversion H.
+Qed.
+
 (*Iterated union*)
 Definition big_union {B: Type} (f: B -> list A) (l: list B) :=
   fold_right (fun x acc => union (f x) acc) nil l.
@@ -95,6 +106,15 @@ Proof.
   clear Heqbase. generalize dependent base.
   induction l; simpl; auto.
   intros base Hbase. apply union_nodup. apply IHl. auto.
+Qed.
+
+Lemma big_union_nil: forall {B: Type} (f: B -> list A) (l: list B),
+  big_union f l = nil ->
+  forall x, In x l -> f x = nil.
+Proof.
+  intros. induction l; simpl in *. inversion H0.
+  apply union_nil in H. destruct H.
+  destruct H0; subst; auto.
 Qed.
 
 End Union.
@@ -164,4 +184,59 @@ Proof.
 Qed.
 
 End Remove.
+
+(* Equality on Lists *)
+
+(* In many cases (particularly those that arise when we have induction principles
+  whose IH involves a list), it is easiest to prove list equality by showing that
+  each element is equal. The following lemmas allow us to do this. *)
+
+Ltac contra :=
+  solve[let C := fresh in
+    intro C; inversion C].
+
+(*We can compare lists elementwise for equality*)
+Lemma list_eq_ext: forall {A: Type} (l1 l2: list A),
+  length l1 = length l2 ->
+  (forall n d, nth n l1 d = nth n l2 d) ->
+  l1 = l2.
+Proof.
+  intros A l1. induction l1 as [|h1 t1 IH]; simpl; intros l2.
+  - destruct l2;[reflexivity | contra].
+  - destruct l2; [contra | intro Heq; inversion Heq; subst].
+    simpl. intros Hnth.
+    assert (h1 = a). {
+      specialize (Hnth 0 h1); apply Hnth.
+    }
+    subst. f_equal. apply IH. assumption.
+    intros n d. specialize (Hnth (S n) d); apply Hnth.
+Qed.
+
+(*In fact, we need only to consider valid indices*)
+Lemma list_eq_ext': forall {A: Type} (l1 l2: list A),
+  length l1 = length l2 ->
+  (forall n d, n < length l1 -> nth n l1 d = nth n l2 d) ->
+  l1 = l2.
+Proof.
+  intros A l1 l2 Hlen Hall. apply list_eq_ext; auto.
+  intros n d. 
+  assert (n < length l1 \/ n >= length l1) by lia.
+  destruct H as [Hin | Hout].
+  - apply Hall. assumption.
+  - rewrite !nth_overflow; try lia. reflexivity.
+Qed.
+
+(*More general than [map_nth] from the standard library because
+  we don't require any knowledge of the default values as long
+  as n is within bounds*)
+Lemma map_nth_inbound: forall {A B: Type} (f: A -> B) (l: list A)
+  (d1 : B) (d2 : A) (n: nat),
+  n < length l ->
+  nth n (List.map f l) d1 = f (nth n l d2).
+Proof.
+  intros A B f l d1 d2. induction l as [|h t IH]; simpl; try lia.
+  intros n Hn.
+  destruct n. reflexivity.
+  apply IH. lia.
+Qed. 
 
